Clean up proofs, add comments

proofs/core/ADTSpec.v
@@ -24,6 +24,29 @@ Goal: sound reasoning about Why3 proof terms via shallowly embedded Rocq terms
   *)
 Require Export Hlist Typing Domain. (*TODO: remove*)
 
+Set Bullet Behavior "Strict Subproofs".
+
+(*TODO MOVE*)
+Lemma list_map_map_In_le {A: Type} (f: A -> nat) {l: list A} {x: A}:
+  In x l ->
+  f x <= list_max (map f l).
+Proof.
+  intros Hin.
+  pose proof (list_max_le (map f l) (list_max (map f l))) as [Hmax _].
+  specialize (Hmax (ltac:(lia))).
+  rewrite Forall_map, Forall_forall in Hmax.
+  auto.
+Qed. 
+
+(*TODO: move*)
+Lemma in_sum_le {A: Type} (f: A -> nat) {l: list A} {x: A}:
+  In x l ->
+  f x <= sum (map f l).
+Proof.
+  induction l as [| h t IH]; simpl; auto; [contradiction|].
+  intros [Hh | Ht]; subst; try lia. specialize (IH Ht); lia.
+Qed.
+
 Definition fun_interp (pd: sort -> Set) := forall (f:funsym) (srts: list sort)
     (a: arg_list (domain pd) (sym_sigma_args f srts)),
     (domain pd (funsym_sigma_ret f srts)).
@@ -91,218 +114,18 @@ Record adt_interp_props {gamma: context} (gamma_valid: valid_context gamma)
     ),
     forall t t_in (x: adt_rep pd t srts), P t t_in x;
   }.
-(* 
+
+(*Construction of a [pi_dom_full] (TODO: maybe move)*)
+
 Require Import IndTypes.
 
-
-(*TODO: move*)
-Definition mk_Forall {A: Type} {P: A -> Prop} := 
-  fun (f: forall x, P x) =>
-    fix mk_Forall (l: list A) {struct l} : Forall P l :=
-      match l with
-      | nil => Forall_nil _
-      | x :: xs => Forall_cons _ _ _ (f x) (mk_Forall xs)
-      end.
-
-Definition mk_ForallT {A: Type} {P: A -> Type} := 
-  fun (f: forall x, P x) =>
-    fix mk_ForallT (l: list A) {struct l} : ForallT P l :=
-      match l with
-      | nil => ForallT_nil _
-      | x :: xs => ForallT_cons _ (f x) (mk_ForallT xs)
-      end.
-
-Unset Elimination Schemes.
-Inductive srt :=
-  | srt_int : srt
-  | srt_real : srt
-  | srt_cons: typesym -> list srt -> srt.
-Set Elimination Schemes.
-
-Fixpoint srt_ind (P: srt -> Prop) (P_int: P srt_int) (P_real: P srt_real) 
-  (P_cons: forall (ts: typesym) (srts: list srt) (IH: Forall P srts), P (srt_cons ts srts))
-  (s: srt) : P s :=
-  match s with
-  | srt_int => P_int
-  | srt_real => P_real
-  | srt_cons ts srts => P_cons ts srts (mk_Forall (srt_ind P P_int P_real P_cons) srts)
-  end.
-
-Fixpoint srt_rect (P: srt -> Type) (P_int: P srt_int) (P_real: P srt_real) 
-  (P_cons: forall (ts: typesym) (srts: list srt) (IH: ForallT P srts), P (srt_cons ts srts))
-  (s: srt) : P s :=
-  match s with
-  | srt_int => P_int
-  | srt_real => P_real
-  | srt_cons ts srts => P_cons ts srts (mk_ForallT (srt_rect P P_int P_real P_cons) srts)
-  end.
-
-Lemma var_not_sort v: ~ is_sort (vty_var v).
-Proof.
-  unfold is_sort. simpl. rewrite aset_singleton_not_empty. auto.
-Qed.
-
-Lemma is_sort_cons_Forall ts l: is_sort (vty_cons ts l) -> Forall is_sort l.
-Proof.
-  rewrite Forall_forall. apply is_sort_cons.
-Qed.
-
-(*The isomorphism*)
-
-Fixpoint sort_to_srt_aux (t: vty) (Hs: is_sort t) : srt :=
-  match t return is_sort t -> srt with
-  | vty_int => fun _ => srt_int
-  | vty_real => fun _ => srt_real
-  | vty_var v => fun Hs => False_rect _ (var_not_sort _ Hs)
-  | vty_cons ts tys => fun Hs => srt_cons ts (dep_map sort_to_srt_aux tys (is_sort_cons_Forall _ _ Hs))
-  end Hs.
-
-Definition sort_to_srt (s: sort) : srt := sort_to_srt_aux (proj1_sig s) (proj2_sig s).
-
-Fixpoint srt_to_ty (s: srt) : vty :=
-  match s with
-  | srt_int => vty_int
-  | srt_real => vty_real
-  | srt_cons ts srts => vty_cons ts (map srt_to_ty srts)
-  end.
-
-Lemma srt_to_ty_sort s: is_sort (srt_to_ty s).
-Proof.
-  induction s; simpl; auto.
-  apply is_sort_cons_iff.
-  rewrite <- Forall_forall, Forall_map.
-  exact IH.
-Qed.
-
-Definition srt_to_sort (s: srt) : sort := exist is_sort _ (srt_to_ty_sort s).
-
-Set Bullet Behavior "Strict Subproofs".
-
-Lemma srt_to_sort_to_srt s:
-  sort_to_srt (srt_to_sort s) = s.
-Proof.
-  unfold sort_to_srt, srt_to_sort. simpl.
-  generalize dependent (srt_to_ty_sort s).
-  induction s; simpl; try reflexivity.
-  intros Hsort. f_equal.
-  generalize dependent (is_sort_cons_Forall ts (map srt_to_ty srts) Hsort).
-  induction srts as [| s stl IHs]; simpl; auto.
-  intros f. inversion IH as [| ? ? Hs Hst]; subst. 
-  f_equal.
-  - apply Hs.
-  - apply IHs; auto. inversion f; subst. 
-    rewrite is_sort_cons_iff, <- Forall_forall.
-    assumption.
-Qed.
-
-Lemma sort_to_srt_to_sort s:
-  srt_to_sort (sort_to_srt s) = s.
-Proof.
-  unfold srt_to_sort, sort_to_srt. apply sort_inj. simpl.
-  destruct s as [ty Hsort]. simpl.
-  revert Hsort.
-  induction ty as [| | v | ts tys IHtys]; simpl; auto.
-  - intros Hsort. exfalso. apply (var_not_sort _ Hsort).
-  - intros Hsort. f_equal. rewrite map_dep_map.
-    generalize dependent (is_sort_cons_Forall ts tys Hsort).
-    clear Hsort. induction tys as [| x tl IHtl]; simpl; auto.
-    intros Hall. inversion IHtys as [| ? ? Hx Htl]; subst.
-    inversion Hall as [| ? ? Hsx Hstl]; subst.
-    f_equal; auto.
-Qed.
-
-Lemma srt_to_sort_int: srt_to_sort srt_int = s_int.
-Proof.
-  apply sort_inj. reflexivity.
-Qed.
-
-Lemma srt_to_sort_real: srt_to_sort srt_real = s_real.
-Proof.
-  apply sort_inj. reflexivity.
-Qed.
-
-Lemma srt_to_sort_cons ts srts: srt_to_sort (srt_cons ts srts) = typesym_to_sort ts (map srt_to_sort srts).
-Proof.
-  apply sort_inj. simpl. f_equal.
-  induction srts as [| x t IH]; simpl; auto.
-  f_equal. auto.
-Qed.
-
-(*And now an induction principle on sorts*)
-Lemma sort_ind (P: sort -> Prop) (P_int: P s_int) (P_real: P s_real)
-  (P_cons: forall (ts: typesym) (srts: list sort) (IH: Forall P srts), P (typesym_to_sort ts srts))
-  (s: sort) : P s.
-Proof.
-  set (s' := sort_to_srt s).
-  set (P' := fun (s: srt) => P (srt_to_sort s)).
-  assert (Hp: P' s'). {
-    apply srt_ind.
-    - unfold P'. rewrite srt_to_sort_int. exact P_int.
-    - unfold P'. rewrite srt_to_sort_real. exact P_real.
-    - intros ts srts. unfold P'. rewrite srt_to_sort_cons. intros Hall. 
-      apply P_cons; rewrite Forall_map; auto.
-  }
-  unfold P', s' in Hp. rewrite sort_to_srt_to_sort in Hp.
-  exact Hp.
-Qed.
-
-(*Note: opaque for now*)
-Lemma ForallT_map1 {A B: Type} (f: A -> B) (P: B -> Type) (l: list A):
-  ForallT P (map f l) -> ForallT (fun x => P (f x)) l.
-Proof.
-  induction l as [| h t IH].
-  - constructor.
-  - intros Hall. inversion Hall; subst. constructor; auto.
-Qed. 
-
-Lemma ForallT_map2 {A B: Type} (f: A -> B) (P: B -> Type) (l: list A):
-  ForallT (fun x => P (f x)) l -> ForallT P (map f l).
-Proof.
-  induction l as [| h t IH].
-  - constructor.
-  - intros Hall. inversion Hall; subst. constructor; auto.
-Qed. 
-
-(*Opaque*)
-Lemma sort_rect (P: sort -> Type) (P_int: P s_int) (P_real: P s_real)
-  (P_cons: forall (ts: typesym) (srts: list sort) (IH: ForallT P srts), P (typesym_to_sort ts srts))
-  (s: sort) : P s.
-Proof.
-  set (s' := sort_to_srt s).
-  set (P' := fun (s: srt) => P (srt_to_sort s)).
-  assert (Hp: P' s'). {
-    apply srt_rect.
-    - unfold P'. rewrite srt_to_sort_int. exact P_int.
-    - unfold P'. rewrite srt_to_sort_real. exact P_real.
-    - intros ts srts. unfold P'. rewrite srt_to_sort_cons. intros Hall. 
-      apply P_cons. apply ForallT_map2. exact Hall.
-  }
-  unfold P', s' in Hp. rewrite sort_to_srt_to_sort in Hp.
-  exact Hp.
-Qed.
-
-(*TODO: just use recursive sort*)
-Lemma sort_rect_int P P_int P_real P_cons:
-  sort_rect P P_int P_real P_cons s_int = P_int.
-Proof. Admitted.
-
-Lemma sort_rect_real P P_int P_real P_cons:
-  sort_rect P P_int P_real P_cons s_real = P_real.
-Proof. Admitted.
-
-Lemma sort_rect_typesym_to_sort P P_int P_real P_cons ts srts:
-  sort_rect P P_int P_real P_cons (typesym_to_sort ts srts) = 
-  P_cons ts srts (mk_ForallT (sort_rect P P_int P_real P_cons) srts).
-Admitted. *)
-
-Require Import IndTypes. (*TODO: move get_nond_vtys?*)
-
+(*We will have to reason about the (ts, tys) pairs that appear as (non-recursive)
+  arguments in ADT constructors. We define the relevant parts below:*)
 Definition vty_ts_pair (t: vty) : option (typesym * list vty) :=
   match t with
   | vty_cons ts vs => Some (ts, vs)
   | _ => None
   end.
-
 
 Definition funsym_ts_pairs m (f: funsym) : list (typesym * list vty) :=
   omap vty_ts_pair (get_nonind_vtys m (s_args f)).
@@ -312,24 +135,35 @@ Definition adt_ts_pairs m a : list (typesym * list vty) :=
 
 Definition mut_ts_pairs m := concat (map (adt_ts_pairs m) m).
 
+(*The construction of the interpretation is very complicated, since it must
+  be defined in terms of itself. There is no obvious recursive argument; instead
+  we use fuel and define a bound. However, in order to reason about this,
+  we need a measure on typesyms, sorts, and tys that satisfies several properties
+  simultaneously:
+  1. If s in srts, |s| <= |srts|
+  2. |srts| < | s_cons ts srts |
+  3. for any (ts, tys) appearing in a constructor of ADT a, and for any sorts,
+     | s_cons ts (sigma tys) | < | s_cons a srts |, where sigma maps the ADT params to srts
 
-Set Bullet Behavior "Strict Subproofs".
+  It is not easy to satisfy these conditions. For example, suppose we have type A a and then
+  type B a that has a constructor taking in A a. By these conditions, it must be the case that:
+  | B int | < | A (B int) | < |B (B int) |
+  This rules out any lexicographic-type approach based on the ordering of typesyms, since
+  A and B are directly comparable.
+  
+  Instead, we need a more complex measure: we define the size of a typesym to be
+  the sum of the sizes of ALL (non-recursive) types appearing in the constructors
+  of the ADTs in the mutual block to which the typesym belongs, and simulateously
+  define the size of a type (for the cons case) as 1 + | ts | + max_{t in ty} | t |.
+  Note that this is self-referrential, so we define via the context.
+  The crucial ingredient to make this well-founded is that types in a context are defined
+  only via previously-defined types (since we consider non-recursive occurrences only).
 
-Lemma list_map_map_In_le {A: Type} (f: A -> nat) {l: list A} {x: A}:
-  In x l ->
-  f x <= list_max (map f l).
-Proof.
-  intros Hin.
-  pose proof (list_max_le (map f l) (list_max (map f l))) as [Hmax _].
-  specialize (Hmax (ltac:(lia))).
-  rewrite Forall_map, Forall_forall in Hmax.
-  auto.
-Qed. 
+  This takes quite a bit of work to show: we define the various size metrics,
+  prove the key lemma that demonstrates the well-foundedness, and then prove the 3 needed results
+*)
 
-
-(*First, the depth measure:*)
-
-Section TestDepth.
+Section Size.
 
 (*To avoid case analysis*)
 Definition is_def_mut (d: def) : option mut_adt :=
@@ -338,12 +172,10 @@ Definition is_def_mut (d: def) : option mut_adt :=
   | _ => None
   end.
 
-
-(*Mutually recursive on typesyms and types*)
+(*The size of a typesym*)
 Fixpoint size_ts (gamma: context) (ts: typesym) :=
   match gamma with
   | nil => 0
-(*   | abs_type t :: g' => if typesym_eq_dec ts t then 1 else size_ts g' ts *)
   | d :: g' =>
     match is_def_mut d with
     | Some m =>
@@ -352,7 +184,7 @@ Fixpoint size_ts (gamma: context) (ts: typesym) :=
         match t with
         | vty_real => 0
         | vty_int => 0
-        | vty_var _ => 0 (*TODO*)
+        | vty_var _ => 0
         | vty_cons ts tys => 1 + size_ts g' ts + list_max (map size_ty tys) (*Crucial: only nonind types!*)
         end in 
       1 + sum (map (fun x => size_ts g' (fst x) + list_max (map size_ty (snd x))) (mut_ts_pairs (adts m)))
@@ -361,21 +193,24 @@ Fixpoint size_ts (gamma: context) (ts: typesym) :=
     end
   end.
 
+(*The size of a type*)
 Fixpoint size_ty (gamma: context) (t: vty) : nat :=
   match t with
   | vty_real => 0
   | vty_int => 0
   | vty_var _ => 0
-  | vty_cons ts tys => 1 + size_ts gamma ts + list_max (map (size_ty gamma) tys) (*Crucial: only nonind types!*)
+  | vty_cons ts tys => 1 + size_ts gamma ts + list_max (map (size_ty gamma) tys)
   end.
 
 Lemma size_ty_cons gamma ts tys:
   size_ty gamma (vty_cons ts tys) = 1 + size_ts gamma ts + list_max (map (size_ty gamma) tys).
 Proof. reflexivity. Qed.
 
+(*The size of a list of types*)
 Definition size_tys (gamma: context) (tys: list vty) : nat :=
   list_max (map (size_ty gamma) tys).
 
+(*A rewrite lemma to avoid the nested fix*)
 Lemma size_ts_rewrite gamma ts:
   size_ts gamma ts =
   match gamma with
@@ -383,7 +218,6 @@ Lemma size_ts_rewrite gamma ts:
   | d :: g' =>
     match is_def_mut d with
     | Some m =>
-(*   | abs_type t :: g' => if typesym_eq_dec ts t then 1 else size_ts g' ts *)
       if in_dec typesym_eq_dec ts (typesyms_of_mut m) then
         1 + sum (map (fun x => size_ts g' (fst x) + list_max (map (size_ty g') (snd x))) (mut_ts_pairs (adts m)))
       else size_ts g' ts
@@ -402,7 +236,7 @@ Proof.
   rewrite Forall_forall in H. auto.
 Qed.
 
-(*And the sort version*)
+(*Size of a sort*)
 Fixpoint size_sort (gamma: context) (s: sort) : nat :=
   match s with
   | s_int => 0
@@ -410,71 +244,49 @@ Fixpoint size_sort (gamma: context) (s: sort) : nat :=
   | s_cons ts srts => 1 + size_ts gamma ts + list_max (map (size_sort gamma) srts)
   end.
 
+(*Size of a list of sorts*)
 Definition size_sorts gamma srts := list_max (map (size_sort gamma) srts).
 
-(*We need a few results*)
-Lemma size_sorts_cons_bound gamma ts srts:
-  size_sorts gamma srts < size_sort gamma (s_cons ts srts).
-Proof.
-  simpl. unfold size_sorts. lia.
-Qed.
+(*The big result: our recursion on the context is justified, and we can instead
+  consider it to have been defined over the entire context*)
+Section Context.
 
-Lemma sort_size_in gamma {s srts}:
-  In s srts ->
-  size_sort gamma s <= size_sorts gamma srts.
-Proof.
-  intros Hin. unfold size_sorts. apply list_map_map_In_le. auto.
-Qed.
+(*We need several helper lemmas first*)
 
-Lemma ty_size_in gamma {t tys}:
-  In t tys ->
-  size_ty gamma t <= size_tys gamma tys.
-Proof.
-  intros Hin. unfold size_tys. apply list_map_map_In_le. auto.
-Qed.
-
-(*We need a bound on substitution: since this calculates depth (i.e the max chain of 
-  typesym size-sums), this is bounded by the sum of the original tys and the substituted sorts
-  (since sorts are substituted at a leaf)*)
-Lemma size_subst_single gamma params srts ty:
-  size_sort gamma (ty_subst_s params srts ty) <= size_ty gamma ty + size_sorts gamma srts.
-Proof.
-  induction ty as [| | x | ts tys IH]; simpl; try lia.
-  - unfold ty_subst_s. simpl.
-    destruct (ty_subst_fun_cases params srts s_int x) as [Hin | Hint].
-    + apply sort_size_in; auto.
-    + rewrite Hint. simpl. lia.
-  - assert (list_max (map (size_sort gamma) (map (v_subst (ty_subst_fun params srts s_int)) tys)) <=
-      list_max (map (size_ty gamma) tys) + size_sorts gamma srts); [|lia].
-    apply list_max_le. rewrite !Forall_map. rewrite Forall_forall in IH |- *. intros x Hinx.
-    specialize (IH x Hinx). unfold ty_subst_s in IH.
-    pose proof (ty_size_in gamma Hinx) as Hle. unfold size_tys in Hle. lia.
-Qed.
-
-Lemma size_subst gamma params srts tys:
-  size_sorts gamma (map (ty_subst_s params srts) tys) <= size_tys gamma tys + size_sorts gamma srts.
-Proof.
-  unfold size_sorts at 1. apply list_max_le.
-  rewrite !Forall_map, Forall_forall. intros x Hinx.
-  pose proof (size_subst_single gamma params srts x) as Hd.
-  pose proof (ty_size_in gamma Hinx). lia.
-Qed.
-
-(*TODO: prove something like: for (ts, tys) in (mut_ts_pairs), ts and all typesyms in tys appear
-  earlier in gamma*)
-
-(*Need an assumption about our types - no nested recursion (TODO: add to typing/valid_context)*)
-(* Lemma size_ty_cons_not_mut g d (Hd: is_def_mut d = None):
-  forall ty, size_ty (d :: g) ty = size_ty g ty.
-Proof.
-  intros ty. induction ty; simpl; auto. *)
-
+(*If d is not a mutual block, size_ts is unaffected*)
 Lemma size_ts_not_mut g d (Hd: is_def_mut d = None):
   forall ts, size_ts (d :: g) ts = size_ts g ts.
 Proof.
   intros ts. rewrite size_ts_rewrite. rewrite Hd. auto.
 Qed.
 
+(*If ts' not in m, then adding d does not change the size of ts'*)
+Lemma size_ts_notin {g d m} (Hd: is_def_mut d = Some m):
+  forall ts' (Hnotin: ~ In ts' (typesyms_of_mut m)),
+  size_ts g ts' = size_ts (d :: g) ts'.
+Proof.
+  intros ts1 Hnotin1. rewrite (size_ts_rewrite (d :: g)), Hd.
+  destruct (in_dec typesym_eq_dec ts1 (typesyms_of_mut m)); auto.
+  contradiction.
+Qed.
+
+(*If no ts in m appears in ty, then size_ty is unaffected by adding d*)
+Lemma size_ty_notin {g d m} (Hd: is_def_mut d = Some m):
+  forall ty
+  (Hnotin: forall ts : typesym, In ts (typesyms_of_mut m) -> ~ is_true (typesym_in_ty ts ty)),
+  size_ty g ty = size_ty (d :: g) ty.
+Proof.
+  intros ty'; induction ty' as [| | x | ts1 tys1 IHty]; auto.
+  intros Hnotin'. rewrite !size_ty_cons, <- !Nat.add_assoc. f_equal.
+  f_equal.
+  - apply (size_ts_notin Hd). intros C. apply (Hnotin' ts1 C). simpl. destruct (typesym_eq_dec ts1 ts1); auto.
+  - f_equal. apply map_ext_in. intros x Hinx.
+    rewrite Forall_forall in IHty. apply IHty; auto. intros ts2 Hints2 C.
+    apply (Hnotin' ts2 Hints2). simpl. apply orb_true_iff. right.
+    rewrite existsb_exists. exists x. auto.
+Qed.
+
+(*Structural result about [mut_ts_pairs]*)
 Lemma mut_ts_pairs_in {m ts tys}:
   In (ts, tys) (mut_ts_pairs (adts m)) ->
   exists a c, adt_in_mut a m /\ constr_in_adt c a /\ In (vty_cons ts tys) (get_nonind_vtys (adts m) (s_args c)).
@@ -491,6 +303,8 @@ Proof.
   - apply In_in_bool; auto.
   - apply constr_in_adt_eq; auto.
 Qed.
+
+(*The following lemmas give us the disjointness results we need*)
 
 (*If (ts, tys) is in the [mut_ts_pairs] list, ts cannot be an adt in m*)
 Lemma mut_ts_pairs_notin_ts {m ts tys}:
@@ -541,7 +355,6 @@ Lemma mut_ts_pairs_in_ctx_valid_type {gamma m ts tys}
 Proof.
   intros Hin. destruct (mut_ts_pairs_in Hin) as [a [c [a_in [c_in Hintys]]]].
   pose proof (wf_context_full _ (valid_context_wf _ gamma_valid)) as [Hwf _].
-  Search funsyms_of_context.
   pose proof (constrs_in_funsyms m_in a_in c_in) as Hinc.
   rewrite Forall_forall in Hwf. specialize (Hwf _ Hinc).
   unfold wf_funsym in Hwf.
@@ -584,6 +397,8 @@ Proof.
   apply (valid_type_typesym_in_ty Hvals); auto.
 Qed.
 
+(*The full theorem:*)
+
 (*Here is where we need the well-founded result: we define only in terms of smaller contexts,
   but this is OK because we look only at nonrecursive references, which must be defined earlier*)
 Lemma size_ts_eq gamma ts:
@@ -617,28 +432,6 @@ Proof.
     - apply size_ts_not_mut; auto.
     - f_equal. apply map_ext. auto.
   }
-  (*Some results helpful for recursive cases. 1. If ts' not in m,
-    then adding d does not change the size of ts' (TODO: separate lemmas?)*)
-  assert (Hnotints: forall ts' (Hnotin: ~ In ts' (typesyms_of_mut m)),
-        size_ts g' ts' = size_ts (d :: g') ts').
-  { intros ts1 Hnotin1. rewrite (size_ts_rewrite (d :: g')), Hmut.
-    destruct (in_dec typesym_eq_dec ts1 (typesyms_of_mut m)); auto.
-    contradiction.
-  }
-  (*2: If no ts in m appears in ty, then size_ty is unaffected by adding d*)
-  assert (Hnotinty: forall ty
-    (Hnotin: forall ts : typesym, In ts (typesyms_of_mut m) -> ~ is_true (typesym_in_ty ts ty)),
-    size_ty g' ty = size_ty (d :: g') ty).
-  {
-    intros ty'; induction ty' as [| | x | ts1 tys1 IHty]; auto.
-    intros Hnotin'. rewrite !size_ty_cons, <- !Nat.add_assoc. f_equal.
-    f_equal.
-    - apply Hnotints. intros C. apply (Hnotin' ts1 C). simpl. destruct (typesym_eq_dec ts1 ts1); auto.
-    - f_equal. apply map_ext_in. intros x Hinx.
-      rewrite Forall_forall in IHty. apply IHty; auto. intros ts2 Hints2 C.
-      apply (Hnotin' ts2 Hints2). simpl. apply orb_true_iff. right.
-      rewrite existsb_exists. exists x. auto.
-  }
   destruct (in_dec typesym_eq_dec ts (typesyms_of_mut m)) as [Hints | Hnotin].
   - (*Case 1: typesym is in mutual type*)
     assert (m_in: mut_in_ctx m (d :: g')). { apply mut_in_ctx_eq.
@@ -654,10 +447,10 @@ Proof.
     (*Now we prove that size_ty and size_ts are the same BECAUSE no types in (mut_ts_pairs) can be in d*)
     apply map_ext_in. intros [ts' tys'] Hin. simpl fst. simpl snd. f_equal.
     + (*Idea: we know that no typesym in d appears in the typesym*)
-      apply Hnotints. apply (mut_ts_pairs_notin_ts Hin); auto. (*contradicts only nonind tys*)
+      apply (size_ts_notin Hmut). apply (mut_ts_pairs_notin_ts Hin); auto. (*contradicts only nonind tys*)
     + (*And similar for the tys*)
       f_equal. apply map_ext_in. intros ty Hinty.
-      apply Hnotinty.  intros ts Hints.
+      apply (size_ty_notin Hmut). intros ts Hints.
       apply (mut_ts_pairs_not_tys Hval' m_in Hin Hinty); auto.
   - (*Case 2: typesym not in mutual type*)
     assert (Hfind: find_ts_in_ctx (d :: g') ts = find_ts_in_ctx g' ts). {
@@ -668,11 +461,11 @@ Proof.
       apply in_map. apply in_bool_In in H; auto.
     }
     rewrite Hfind, IH.
-    clear Hfind.
+    clear Hfind IH.
     destruct (find_ts_in_ctx g' ts) as [[m1 a1]|] eqn : Hfind; auto.
     f_equal. f_equal.
     (*Now we have a similar proof, but now we know that because they are defined before,
-      they can only refer to names that came before (TODO: prove)*)
+      they can only refer to names that came before*)
     apply find_ts_in_ctx_some in Hfind. destruct Hfind as [m1_in [a1_in Hts]].
     (*Common in both cases: anything previously defined in the context cannot
       overlap with a definition in m*)
@@ -688,36 +481,69 @@ Proof.
       rewrite in_app_iff. right. apply in_map; auto.
     }
     apply map_ext_in. intros [ts' tys'] Hin. simpl fst. simpl snd. f_equal.
-    + apply Hnotints. (*by [mut_ts_pairs_ts_in_ctx], ts' is in sig_t of g',
+    + apply (size_ts_notin Hmut). 
+      (*by [mut_ts_pairs_ts_in_ctx], ts' is in sig_t of g',
       so it will contradict disjointness*)
       pose proof (mut_ts_pairs_ts_in_ctx Hval m1_in Hin) as Hints.
       apply Hdisj'; auto.
     + (*Similarly, no ts in m can appear in tys'*) f_equal. apply map_ext_in. intros a Hina.
-      apply Hnotinty.
+      apply (size_ty_notin Hmut).
       intros ts1 Hints1 Hinty.
       apply (Hdisj' ts1); auto.
       apply (mut_ts_pairs_in_tys_in_ctx Hval m1_in Hin _ _ Hina); auto.
 Qed.
 
-(* 
-Lemma size_ts_rewrite gamma ts:
-  size_ts gamma ts =
-  match gamma with
-  | nil => 0
-  | abs_type t :: g' => if typesym_eq_dec ts t then 1 else size_ts g' ts
-  | datatype_def m :: g' => if in_dec typesym_eq_dec ts (typesyms_of_mut m) then
-      1 + sum (map (fun x => size_ty g' (vty_cons (fst x) (snd x))) (mut_ts_pairs (adts m)))
-    else size_ts g' ts
-  | _ :: g' => size_ts g' ts
-  end.
- *)
+End Context.
 
-Lemma in_sum_le {A: Type} (f: A -> nat) {l: list A} {x: A}:
-  In x l ->
-  f x <= sum (map f l).
+(*Now we prove the bounds via this measure*)
+Section Bounds.
+
+Lemma size_sorts_cons_bound gamma ts srts:
+  size_sorts gamma srts < size_sort gamma (s_cons ts srts).
 Proof.
-  induction l as [| h t IH]; simpl; auto; [contradiction|].
-  intros [Hh | Ht]; subst; try lia. specialize (IH Ht); lia.
+  simpl. unfold size_sorts. lia.
+Qed.
+
+Lemma sort_size_in gamma {s srts}:
+  In s srts ->
+  size_sort gamma s <= size_sorts gamma srts.
+Proof.
+  intros Hin. unfold size_sorts. apply list_map_map_In_le. auto.
+Qed.
+
+Lemma ty_size_in gamma {t tys}:
+  In t tys ->
+  size_ty gamma t <= size_tys gamma tys.
+Proof.
+  intros Hin. unfold size_tys. apply list_map_map_In_le. auto.
+Qed.
+
+(*Substitution is the trickiest. The idea is that, since the type size ultimately calculates
+  depth (i.e. the max chain of typesym size-sums), we can bound a substitution by a sum of
+  the original tys and the substituted sorts (since sorts are substituted at a leaf)*)
+
+Lemma size_subst_single gamma params srts ty:
+  size_sort gamma (ty_subst_s params srts ty) <= size_ty gamma ty + size_sorts gamma srts.
+Proof.
+  induction ty as [| | x | ts tys IH]; simpl; try lia.
+  - unfold ty_subst_s. simpl.
+    destruct (ty_subst_fun_cases params srts s_int x) as [Hin | Hint].
+    + apply sort_size_in; auto.
+    + rewrite Hint. simpl. lia.
+  - assert (list_max (map (size_sort gamma) (map (v_subst (ty_subst_fun params srts s_int)) tys)) <=
+      list_max (map (size_ty gamma) tys) + size_sorts gamma srts); [|lia].
+    apply list_max_le. rewrite !Forall_map. rewrite Forall_forall in IH |- *. intros x Hinx.
+    specialize (IH x Hinx). unfold ty_subst_s in IH.
+    pose proof (ty_size_in gamma Hinx) as Hle. unfold size_tys in Hle. lia.
+Qed.
+
+Lemma size_subst gamma params srts tys:
+  size_sorts gamma (map (ty_subst_s params srts) tys) <= size_tys gamma tys + size_sorts gamma srts.
+Proof.
+  unfold size_sorts at 1. apply list_max_le.
+  rewrite !Forall_map, Forall_forall. intros x Hinx.
+  pose proof (size_subst_single gamma params srts x) as Hd.
+  pose proof (ty_size_in gamma Hinx). lia.
 Qed.
 
 (*Now this is why we needed the convoluted method of computing the size of a typesym:
@@ -744,7 +570,7 @@ Proof.
   unfold size_sorts. reflexivity.
 Qed.
 
-
+(*And therefore, we get condition (3) above*)
 Lemma mut_ts_pairs_subst_smaller {gamma m a} (gamma_valid: valid_context gamma) (m_in: mut_in_ctx m gamma)
   (a_in: adt_in_mut a m) ts' tys' srts
   (Hin: In (ts', tys') (mut_ts_pairs (adts m))):
@@ -756,124 +582,8 @@ Proof.
   pose proof (mut_ts_pairs_size gamma_valid m_in a_in Hin). lia.
 Qed.
 
-End TestDepth.
-
-
-Definition ts_map_to_pd (f: typesym -> list sort -> Set) : sort -> Set :=
-  fun s =>
-  match s with
-  | s_int => Z
-  | s_real => R
-  | s_cons ts srts => f ts srts
-  end.
-
-(* Lemma ts_map_to_pd_domain f:
-   *)
-
-Require Import IndTypes.
-
-Definition adt_rep' (m: mut_adt) (srts: list sort) (d1 d2: sort -> Set) (a: alg_datatype)
-  (a_in: adt_in_mut a m) :=
-  mk_adts (var_map m srts d1) (typesym_map m srts d2) (adts m) (get_idx adt_dec a (adts m) a_in).
-
-Fixpoint mk_ts_map (gamma: context) (pd: sort -> Set) (n: nat) (ts: typesym) (srts: list sort) : Set :=
-  match n with
-  | O => pd (s_cons ts srts)
-  | S n' =>
-    let pd' := ts_map_to_pd (mk_ts_map gamma pd n')
-(*     sort_rect (fun _ => Set) Z R (fun ts srts IH => mk_ts_map gamma n' pd ts srts) *)
-     (*  let fix f (s: srt) : Set :=
-      match s with
-      | srt_int => Z
-      | srt_real => R
-      | srt_cons ts srts => mk_ts_map gamma n' f ts (map srt_to_sort srts)
-      end in
-      f (sort_to_srt s) *)
-    in
-    match find_ts_in_ctx gamma ts as b return find_ts_in_ctx gamma ts = b -> _ with
-    | Some (m, a) => fun Hfind => adt_rep m srts pd' a (proj1 (proj2 (find_ts_in_ctx_some _ _ _ _ Hfind)))
-    | None => fun _ => pd (s_cons ts srts)
-    end eq_refl
-    end.
-
-Definition mk_pd_aux (gamma: context) (pd: sort -> Set) (n: list sort -> nat) (s: sort) : Set :=
-  ts_map_to_pd (fun ts srts => mk_ts_map gamma pd (n srts) ts srts) s.
-
-(*Idea: should be invariant as long as n larger than max depth of sort*)
-Fixpoint sort_depth (n: typesym -> nat) (s: sort) : nat :=
-  match s with
-  | s_int => 1
-  | s_real => 1
-  | s_cons ts srts => 1 + n ts * list_max (map (sort_depth n) srts)
-  end.
-
-Definition sorts_depth n (s: list sort) : nat := list_max (map (sort_depth n) s).
-
-
-Definition funsym_vars (f: funsym) : aset typevar :=
-  aset_big_union type_vars (s_args f).
-Definition adt_vars (a: alg_datatype) : aset typevar :=
-  aset_big_union funsym_vars (adt_constr_list a).
-Definition mut_vars (l: list (alg_datatype)) : aset typevar :=
-  aset_big_union adt_vars l.
-
-
-(*The total bound, with var bound given by n*)
-(* Fixpoint vty_size (n: typesym -> nat) (v: vty) :=
-  match v with
-  | vty_int => 1
-  | vty_real => 1
-  | vty_var _ => 1
-  | vty_cons t ts => 1 + (n t) * list_max (map (vty_size n) ts)
-  end.
-
-
-Definition constr_depth (gamma:context) :=
-  1 + list_max (map (fun x => 1 + list_max (map ((vty_size (fun ts => index typesym_eq_dec ts (typesyms_of_context gamma))))
-  (snd x))) (mut_ts_pairs (adts_of_context gamma))).
-
-Lemma constr_depth_pos gamma: constr_depth gamma >= 1.
-Proof. unfold constr_depth. lia. Qed.
-
-Definition depth_aux gamma s :=
-  sort_depth (fun ts => (index typesym_eq_dec ts (typesyms_of_context gamma)) * (constr_depth gamma)) s.
-
-Definition depth gamma srts :=
-  list_max (map (depth_aux gamma) srts). *)
-
-
-Fixpoint depth_alt gamma s :=
-   match s with
-  | s_int => 0
-  | s_real => 0
-  | s_cons ts srts =>
-       1 + ((index typesym_eq_dec ts (typesyms_of_context gamma))) + 
-      list_max (map (depth_alt gamma) srts)
-      (* max ((index typesym_eq_dec ts (typesyms_of_context gamma)))
-      (list_max (map (depth_alt gamma) srts)) *)
-  end.
-
-Definition depth gamma srts :=
-  list_max (map (depth_alt gamma) srts).
-
-
-Definition mk_ts_full gamma pd ts srts :=
-  mk_ts_map gamma pd (size_sorts gamma srts) ts srts.
-
-Print index.
-
-Definition max_depth gamma srts :=
-  3 + list_max (map (size_ts gamma) (typesyms_of_context gamma)) + size_sorts gamma srts.
-(*   3 + (length (typesyms_of_context gamma)) + max (length (typesyms_of_context gamma)) (depth gamma srts). *)
-
-Lemma index_leq_length {A: Type} eq_dec (x: A) (l: list A):
-  index eq_dec x l <= length l.
-Proof.
-  induction l; simpl; auto.
-  destruct (eq_dec _ _); lia.
-Qed.
-
-(*TODO: move above*)
+(*We need one more result: any typesym not in the context has size 0
+  (NOTE: this cannot depend on [valid_context]*)
 Lemma ts_notin_size {gamma ts}:
   ~ In ts (typesyms_of_context gamma) ->
   size_ts gamma ts = 0.
@@ -893,6 +603,53 @@ Proof.
   - destruct d; try discriminate; simpl in Hnotin; auto.
 Qed. 
 
+End Bounds.
+End Size.
+
+(*Part 2: Define the interp
+
+This is not easy, since it must be defined in terms of itself. Even the fuel can change during
+recursive calls, since it is a function of the input sort/sorts. In a sense, the fuel is variable,
+and then gets "fixed" and treated as a normal [nat] for the rest of the recursion. We need appropriate
+bounds to ensure that this works, but it is very tricky.
+*)
+
+Definition ts_map_to_pd (f: typesym -> list sort -> Set) : sort -> Set :=
+  fun s =>
+  match s with
+  | s_int => Z
+  | s_real => R
+  | s_cons ts srts => f ts srts
+  end.
+
+(*The core map: sends typesyms in the context to the correct [adt_rep].
+  But for well-founded recursion, the [adt_rep] is defined in terms of a smaller fuel bound.
+  Proving that we can ultimately equate this with the input [nat] (for large enough n)
+  is the key challenge*)
+Fixpoint mk_ts_map (gamma: context) (pd: sort -> Set) (n: nat) (ts: typesym) (srts: list sort) : Set :=
+  match n with
+  | O => pd (s_cons ts srts)
+  | S n' =>
+    let pd' := ts_map_to_pd (mk_ts_map gamma pd n')
+    in
+    match find_ts_in_ctx gamma ts as b return find_ts_in_ctx gamma ts = b -> _ with
+    | Some (m, a) => fun Hfind => adt_rep m srts pd' a (proj1 (proj2 (find_ts_in_ctx_some _ _ _ _ Hfind)))
+    | None => fun _ => pd (s_cons ts srts)
+    end eq_refl
+    end.
+
+(*The [pi_dom] defined with function for the size (based on input sorts)*)
+Definition mk_pd_aux (gamma: context) (pd: sort -> Set) (n: list sort -> nat) (s: sort) : Set :=
+  ts_map_to_pd (fun ts srts => mk_ts_map gamma pd (n srts) ts srts) s.
+
+Definition mk_ts_full gamma pd ts srts :=
+  mk_ts_map gamma pd (size_sorts gamma srts) ts srts.
+
+(*Given a [srts], we need a max depth of any (s_cons ts srts). This is easy: just take the largest
+  size typesym in the context (all others are 0) *)
+Definition max_depth gamma srts :=
+  3 + list_max (map (size_ts gamma) (typesyms_of_context gamma)) + size_sorts gamma srts.
+
 Lemma max_depth_max gamma:
   forall ts srts, 1 + size_sort gamma (s_cons ts srts) < max_depth gamma srts.
 Proof.
@@ -903,9 +660,11 @@ Proof.
   - rewrite ts_notin_size; auto. lia.
 Qed. 
 
+(*The complete interpretation: give [max_depth gamma srts] as the fuel bound for each [srts]*)
 Definition mk_pd (gamma: context) (pd: sort -> Set) (s: sort) : Set :=
   mk_pd_aux gamma pd (fun srts => max_depth gamma srts) s.
 
+(*Definitions of correctness:*)
 
 (*pd with all typesym_to_sort set correctly to the corresponidng W-type*)
 Definition pd_full (gamma: context) (pd: sort -> Set) := forall (m: mut_adt) (srts: list sort)
@@ -913,33 +672,18 @@ Definition pd_full (gamma: context) (pd: sort -> Set) := forall (m: mut_adt) (sr
     pd (s_cons (adt_name a) srts) =
     adt_rep m srts pd a Hin.
 
+(*The auxillary version. The [n] function must be large enough*)
 Definition pd_full_aux (gamma: context) (pd: sort -> Set) (n: list sort -> nat) := 
     (forall ts srts1, 1 + size_sort gamma (s_cons ts srts1) < n srts1) ->
     forall (m: mut_adt) (srts: list sort)
     (a: alg_datatype) (m_in: mut_in_ctx m gamma) (Hin: adt_in_mut a m) ,
     pd (s_cons (adt_name a) srts) =
     adt_rep m srts pd a Hin.
-(* 
-(*TODO: move this*)
-Print mk_adts.
 
-(*Get vars in mutual datatype (note: by well-typing, should be in m_params m)*)
-Print alg_datatype.
-
-Print funsym.
-Print fpsym.
-Print f_sym. *)
-
-
-(*Lemma W_ext (I: Set) (A1 A2: I -> Set) (B1 B2:  *)
-
-(*Lemma big_sprod_inj l1 l2:
-  big_sprod l1 = big_sprod l2 ->
-  *)
-
-(*TODO: move - this is the key lemma that lets us change interps!*)
+(*TODO: move*)
+(*This is the key lemma that lets us change the intepretation of an [adt_rep]:
+  if the two interpretations agree on all types in the constructors of [m].*)
 Lemma mk_adts_ext v a1 a2 m
-  (*(Hv: forall v, aset_mem v (mut_vars m) -> v1 v = v2 v)*)
   (Ht: forall ts tys, In (ts, tys) (mut_ts_pairs m) -> a1 ts tys = a2 ts tys):
   mk_adts v a1 m = mk_adts v a2 m.
 Proof.
@@ -1016,202 +760,13 @@ Proof.
     intros y Hiny. apply Hall. rewrite Hiny, orb_true_r; auto.
 Qed.
 
-
-Print sort_depth.
-Lemma sort_depth_cons n ts srts:
-  sort_depth n (s_cons ts srts) = 1 + n ts * sorts_depth n srts.
-Proof. reflexivity. Qed.
-
-(*Hmm, not sure if this is true*)
-(*TODO: can remove 1+ if we make depth of int 0 (I think)*)
-(* Lemma sort_depth_subst n params srts x:
-  sort_depth n (ty_subst_s params srts x) <= 1 + (vty_size n x) * (sorts_depth n srts).
-Proof.
-  induction x as [| | x | ts tys IH]; simpl; try lia.
-  - unfold ty_subst_s. simpl.
-    destruct (ty_subst_fun_cases params srts s_int x) as [Hin | Hint].
-    + rewrite Nat.add_0_r. unfold sorts_depth.
-      apply (list_map_map_In_le (sort_depth n)) in Hin. lia.
-    + rewrite Hint. simpl. lia.
-  - apply le_n_S. rewrite map_map.
-    assert (list_max (map (fun x : vty => sort_depth n (v_subst (ty_subst_fun params srts s_int) x)) tys) <= 
-      1 + list_max (map (vty_size n) tys) * sorts_depth n srts).
-    { apply list_max_le. rewrite Forall_map. revert IH. apply Forall_impl_strong. intros a Hina Hle.
-      unfold ty_subst_s in Hle.
-      assert (vty_size n a <= list_max (map (vty_size n) tys)). {
-        apply list_map_map_In_le. auto.
-      }
-      nia.
-    }
-    Admitted. *)
-(*     
-Lemma sorts_depth_sigma gamma m ts tys (m_in: mut_in_ctx m gamma) n srts
-  (Hin: In (ts, tys) (mut_ts_pairs (adts m))):
-  sorts_depth n (map (ty_subst_s (m_params m) srts) tys) <=
-  1 + constr_depth gamma * sorts_depth n srts.
-Proof.
-  unfold sorts_depth.
-  rewrite !map_map.
-  apply list_max_le.
-  rewrite Forall_map, Forall_forall. intros x Hinx.
-
-
-
-  Search list_max (_ <= _).
-
- 
-  induction tys as [| t1 tys IHty]; simpl; try lia. *)
-  
-
-
-(*What about: in typesym to sort (ONLY) can be lexicographic
-  no, not true -only at top level
-  should depend on index
-  cannot keep going forever - idea: eventually get to ADT that has no previously defined typesyms*)
-
-
-(*Test*)
 Require Import Stdlib.Arith.Wf_nat.
 
+Section InterpProofs.
 
-(* 
-
-Lemma mut_ts_pairs_subst_smaller {gamma m a} (gamma_valid: valid_context gamma) n (m_in: mut_in_ctx m gamma)
-  (a_in: adt_in_mut a m) ts' tys' srts
-  (Hn: n >= depth_tys gamma 
-  (Hin: In (ts', tys') (mut_ts_pairs (adts m))):
-
-
-
-Lemma depth_alt_in gamma n {s srts}:
-  In s srts ->
-  depth_alt gamma n s <= depth gamma n srts.
-Proof.
-  intros Hin. unfold depth. 
-  apply list_map_map_In_le; auto.
-Qed. *)
-
-  
-
-(* 
-
-
-
-Fixpoint depth_alt gamma n s :=
-   match s with
-  | s_int => 0
-  | s_real => 0
-  | s_cons ts srts =>
-       1 + (n * ((index typesym_eq_dec ts (typesyms_of_context gamma)))) + 
-      list_max (map (depth_alt gamma n) srts)
-      (* max ((index typesym_eq_dec ts (typesyms_of_context gamma)))
-      (list_max (map (depth_alt gamma) srts)) *)
-  end.
-
-Definition depth gamma n srts :=
-  list_max (map (depth_alt gamma n) srts). *)
-(* 
-Lemma depth_alt_cons_bound gamma n ts srts:
-  depth gamma n srts < depth_alt gamma n (s_cons ts srts).
-Proof.
-  simpl.
-  unfold depth. lia.
-Qed.
-
-Lemma depth_alt_in gamma n {s srts}:
-  In s srts ->
-  depth_alt gamma n s <= depth gamma n srts.
-Proof.
-  intros Hin. unfold depth. 
-  apply list_map_map_In_le; auto.
-Qed. *)
-(* 
-Fixpoint depth_ty (gamma: context) n (ty: vty) : nat :=
-  match ty with
-  | vty_cons ts tys => 
-    1 + (n * index typesym_eq_dec ts (typesyms_of_context gamma)) +
-      (list_max (map (depth_ty gamma n) tys))
-      (* Init.Nat.max (index typesym_eq_dec ts (typesyms_of_context gamma))
-        (list_max (map (depth_ty gamma) tys)) *)
-  | _ => 0
-  end.
-
-Definition depth_tys gamma n tys :=
-  list_max (map (depth_ty gamma n) tys).
-
-Lemma depth_ty_in gamma n {t tys}:
-  In t tys ->
-  depth_ty gamma n t <= depth_tys gamma n tys.
-Proof.
-  intros Hin. unfold depth. 
-  apply list_map_map_In_le; auto.
-Qed.
-
-
-(*Let's just try*)
-Lemma depth_subst_single gamma n params srts ty:
-  depth_alt gamma n (ty_subst_s params srts ty) <= depth_ty gamma n ty + (depth gamma n srts).
-Proof.
-  induction ty as [| | x | ts tys IH]; simpl; try lia.
-  - unfold ty_subst_s. simpl.
-    destruct (ty_subst_fun_cases params srts s_int x) as [Hin | Hint].
-    + apply depth_alt_in; auto.
-    + rewrite Hint. simpl. lia.
-  - assert (list_max (map (depth_alt gamma n) (map (v_subst (ty_subst_fun params srts s_int)) tys)) <=
-      list_max (map (depth_ty gamma n) tys) + depth gamma n srts); [|lia].
-    apply list_max_le. rewrite !Forall_map. rewrite Forall_forall in IH |- *. intros x Hinx.
-    specialize (IH x Hinx). unfold ty_subst_s in IH.
-    pose proof (depth_ty_in gamma n Hinx) as Hle. unfold depth_tys in Hle. lia.
-Qed.
-
-Lemma depth_subst gamma n params srts tys:
-  depth gamma n (map (ty_subst_s params srts) tys) <= depth_tys gamma n tys + (depth gamma n srts).
-Proof.
-  unfold depth at 1. apply list_max_le.
-  rewrite !Forall_map, Forall_forall. intros x Hinx.
-  pose proof (depth_subst_single gamma n params srts x) as Hd.
-  pose proof (depth_ty_in gamma n Hinx). lia.
-Qed.
-
-Lemma mut_ts_pairs_subst_smaller {gamma m a} (gamma_valid: valid_context gamma) n (m_in: mut_in_ctx m gamma)
-  (a_in: adt_in_mut a m) ts' tys' srts
-  (Hn: n >= depth_tys gamma 
-  (Hin: In (ts', tys') (mut_ts_pairs (adts m))):
-  depth_alt gamma n (s_cons ts' (map (ty_subst_s (m_params m) srts) tys')) <
-  depth_alt gamma n (s_cons (adt_name a) srts).
-Proof.
-  simpl.
-  assert (Hts: index typesym_eq_dec ts' (typesyms_of_context gamma) < 
-    index typesym_eq_dec (adt_name a) (typesyms_of_context gamma)). { admit. }
-  pose proof (depth_subst gamma n (m_params m) srts tys') as Hsubst.
-  
-  
-
-  assert (Hsubst: (list_max (map (depth_alt gamma) (map (ty_subst_s (m_params m) srts) tys'))) <=
-    max (list_max (map (depth_alt gamma) srts)) (list_max (map (depth_ty gamma) tys'))).
-  { admit. }
-  (*Problem: NOT index*)
-  Print depth_alt.
-  assert (Htys: (list_max (map (depth_ty gamma) tys') <= 
- *)
-(*  Admitted. *)
-(*Idea: index of ts' is smaller than index of ts, and indices in tys' MUST be 
-      smaller than index of ts as well (by well-typed context)
-      and obviously everythign in srts smaller than srts, so I think we are good
-      *)
-    (* apply PeanoNat.lt_S_n in Hn1, Hn2.
-    assert ( Hindex: index typesym_eq_dec ts' (typesyms_of_context gamma) < 
-      index typesym_eq_dec ts (typesyms_of_context gamma)). { admit. } *)
-    (*Idea: (list_max (map (depth_alt gamma) (map (sigma m srts) tys'))) <=
-      max (list_max (map (depth_alt gamma) srts)) (list_max (map (depth_vty gamma) tys'))
-      by subst properties (maybe we need assumption about params in bounds but that is OK*)
-    (*Then, have that (list_max (map (depth_vty gamma) tys') <= (index typesym_eq_dec ts') by 
-        well-typing of constructors (need valid context) *)
-    (*So, max (index ts') (max (list_map srts) (index ts')) = max (index ts') (max (list_map srts))*)
-    (*And we know that index ts' < index ts', so the result follows*)
-    (*I believe that this should work*)
-
-(*Maybe: prove 2 things: non-dependent and dependent versions*)
+(*The key result is that if the fuel is large enough, the interpretation is independent of
+  the fuel. But we need both non-dependent (constant nat) and (sort -> nat) function versions,
+  and a hybrid. The non-dependent version is the crucial one which we build the others atop.*)
 
 Lemma mk_ts_map_invar_const {gamma} (gamma_valid: valid_context gamma) pd n1 n2 (s: sort):
   size_sort gamma s < n1 ->
@@ -1227,10 +782,11 @@ Proof.
   intros H. generalize dependent (proj1 (proj2 (H m a eq_refl))).
   specialize (H m a eq_refl). destruct H as [m_in [a_in Hts]].
   intros a_in'. assert (a_in' = a_in) by (apply bool_irrelevance); subst.
-  (*TODO: separate lemma*) unfold adt_rep.
+  (*Prove the [adt_rep]s equal by proving the var maps equal and then
+    using the ext lemma for the typesym interp*)
+  unfold adt_rep.
   assert (Hveq: (var_map m srts (ts_map_to_pd (mk_ts_map gamma pd n1))) = 
     (var_map m srts (ts_map_to_pd (mk_ts_map gamma pd n2)))). {
-    (*This should be separate lemma*)
     apply functional_extensionality. intros x.
     unfold var_map. unfold domain. unfold sigma. simpl. unfold ty_subst_s.
     simpl. 
@@ -1241,36 +797,22 @@ Proof.
       simpl in Hn1, Hn2.
       pose proof (list_map_map_In_le (size_sort gamma) Hin).
       apply IHn1; lia.
-      
-(*       admit. *)
-      (* unfold depth_aux in Hn1, Hn2.
-      simpl in Hn1.
-      simpl sort_depth in Hn1, Hn2.
-      assert (Hn1': list_max (map (sort_depth (constr_depth gamma)) srts) < n1) by nia.
-      assert (Hn2': list_max (map (sort_depth (constr_depth gamma)) srts) < n2) by nia.
-      pose proof (list_map_map_In_le (sort_depth (constr_depth gamma)) Hin). *)
-(*       apply IHn1; lia. *)
     + rewrite Hd; auto.
   }
   rewrite Hveq.
   (*Now prove typesym_map equality*)
   erewrite mk_adts_ext; [reflexivity|].
   intros ts' tys' Hin'. unfold typesym_map.
-  (*So we know (if we change bounds) that sort depth is smaller*)
+  (*This is why we need the particular bound: since we are in a constructor
+    argument type, it is smaller than the original sort*)
   unfold domain. simpl.
   specialize (IHn1 (s_cons ts' (map (sigma m srts) tys')) n2).
-(*   simpl sort_depth in Hn1, Hn2. *)
-  (*Know here that ts' is NON-recursive instance - so it MUST appear BEFORE in gamma*)
-(*  apply PeanoNat.lt_S_n in Hn1, Hn2. *)
   pose proof (mut_ts_pairs_subst_smaller gamma_valid m_in a_in ts' tys' srts Hin').
   apply IHn1; unfold sigma; lia.
 Qed.
 
-(*Definition depth_func (gamma: context) (s: sort)*)
-(*TODO: need to figure out if other version (with fixed nat) is enough?*)
+(*The function version*)
 Lemma mk_ts_map_invar {gamma} (gamma_valid : valid_context gamma) pd n1 n2 (s: sort):
-  (* (forall srts, 0 < n1 srts) ->
-  (forall srts, 0 < n2 srts) -> *)
   (forall ts srts, size_sort gamma (s_cons ts srts) < n1 srts) ->
   (forall ts srts, size_sort gamma (s_cons ts srts) < n2 srts) ->
   ts_map_to_pd (fun ts srts => mk_ts_map gamma pd (n1 srts) ts srts) s = 
@@ -1281,10 +823,8 @@ Proof.
   simpl ts_map_to_pd in Heq. apply Heq; auto.
 Qed.
 
-
+(*One side is function, the other is a constant*)
 Lemma mk_ts_map_invar'  {gamma} (gamma_valid : valid_context gamma) pd n1 n2 (s: sort):
-  (* (forall srts, 0 < n1 srts) ->
-  (forall srts, 0 < n2 srts) -> *)
   (forall ts srts, size_sort gamma (s_cons ts srts) < n1 srts) ->
   (size_sort gamma s < n2) ->
   ts_map_to_pd (fun ts srts => mk_ts_map gamma pd (n1 srts) ts srts) s = 
@@ -1294,553 +834,20 @@ Proof.
   pose proof (mk_ts_map_invar_const gamma_valid pd (n1 srts) n2 (s_cons ts srts)) as Heq.
   simpl ts_map_to_pd in Heq. apply Heq; auto.
 Qed.
- (*  simpl.
 
-   assert (Hn1' := Hn1 srts).
-  assert (Hn2' := Hn2 srts).
-  destruct (n1 srts) as [|n1'] eqn : Hn1s; [lia|].
-  destruct (n2 srts) as [|n2'] eqn : Hn2s; [lia|].
-  simpl.
-  generalize dependent (find_ts_in_ctx_some gamma ts).
-  destruct (find_ts_in_ctx gamma ts) as [[m a]|] eqn : Hfind; auto.
-  intros H. generalize dependent (proj1 (proj2 (H m a eq_refl))).
-  specialize (H m a eq_refl). destruct H as [m_in [a_in Hts]].
-  intros a_in'. assert (a_in' = a_in) by (apply bool_irrelevance). subst. 
-  unfold adt_rep.
-
-
-  revert n1 n2.
-  remember (depth_alt gamma s) as n.
-  generalize dependent s.
-  induction n using lt_wf_ind.
-  assert (IH: forall s: sort,
-    depth_alt gamma s < n ->
-    forall n1 n2,
-    (forall srts, 0 < n1 srts) ->
-    (forall srts, 0 < n2 srts) ->
-    (*(forall srts : list sort, depth gamma srts < n1 srts) ->
-    (forall srts : list sort, depth gamma srts < n2 srts) ->*)
-    ts_map_to_pd (fun (ts : typesym) (srts : list sort) => mk_ts_map gamma pd (n1 srts) ts srts) s =
-    ts_map_to_pd (fun (ts : typesym) (srts : list sort) => mk_ts_map gamma pd (n2 srts) ts srts) s).
-  { intros s Hn. apply H with (m:=depth_alt gamma s); auto. }
-  clear H.
-  intros s Hn n1 n2 Hn1 Hn2. subst.
-  destruct s as [| | ts srts]; simpl; auto.
-  assert (Hn1' := Hn1 srts).
-  assert (Hn2' := Hn2 srts).
-  destruct (n1 srts) as [|n1'] eqn : Hn1s; [lia|].
-  destruct (n2 srts) as [|n2'] eqn : Hn2s; [lia|].
-  simpl.
-  generalize dependent (find_ts_in_ctx_some gamma ts).
-  destruct (find_ts_in_ctx gamma ts) as [[m a]|] eqn : Hfind; auto.
-  intros H. generalize dependent (proj1 (proj2 (H m a eq_refl))).
-  specialize (H m a eq_refl). destruct H as [m_in [a_in Hts]].
-  intros a_in'. assert (a_in' = a_in) by (apply bool_irrelevance). subst. 
-  unfold adt_rep.
-  assert (Hveq: (var_map m srts (ts_map_to_pd (mk_ts_map gamma pd n1'))) = 
-    (var_map m srts (ts_map_to_pd (mk_ts_map gamma pd n2')))). {
-    (*This should be separate lemma*)
-    apply functional_extensionality. intros x.
-    unfold var_map. unfold domain. unfold sigma. unfold ty_subst_s.
-    simpl. 
-    destruct (ty_subst_fun_cases (m_params m) srts s_int x) as [Hin | Hd].
-    + remember (ty_subst_fun (m_params m) srts s_int x) as t.
-      destruct (sort_to_ty t) eqn : Hs; auto.
-      { (*sort not var*) destruct t; simpl in Hs; discriminate. }
-      (*We have to change n1 and n2, but we use the fact that it is bounded (I hope)*)
-      pose proof (depth_alt_in gamma Hin).
-      pose proof (depth_alt_cons_bound gamma (adt_name a) srts).
-      apply (IH t); auto; try lia.
-    + rewrite Hd; auto.
-  }
-  rewrite Hveq.
-  (*Now prove typesym_map equality*)
-  erewrite mk_adts_ext; [reflexivity|].
-  intros ts' tys' Hin'. unfold typesym_map.
-  (*So we know (if we change bounds) that sort depth is smaller*)
-  unfold domain. simpl.
-  specialize (IH (s_cons ts' (map (sigma m srts) tys'))).
-  simpl ts_map_to_pd in IH.
-  assert (Hdepth: depth_alt gamma (s_cons ts' (map (sigma m srts) tys')) < depth_alt gamma (s_cons (adt_name a) srts)).
-  {
-    (*Idea: (list_max (map (depth_alt gamma) (map (sigma m srts) tys'))) <=
-      max (list_max (map (depth_alt gamma) srts)) (list_max (map (depth_vty gamma) tys'))
-      by subst properties (maybe we need assumption about params in bounds but that is OK*)
-    (*Then, have that (list_max (map (depth_vty gamma) tys') <= (index typesym_eq_dec ts') by 
-        well-typing of constructors (need valid context) *)
-    (*So, max (index ts') (max (list_map srts) (index ts')) = max (index ts') (max (list_map srts))*)
-    (*And we know that index ts' < index ts', so the result follows*)
-    (*I believe that this should work*)
-    admit.
-  }
-  specialize (IH Hdepth (fun _ => n1') (fun _ => n2')).
-(*   simpl sort_depth in Hn1, Hn2. *)
-  (*Know here that ts' is NON-recursive instance - so it MUST appear BEFORE in gamma*)
-(*  apply PeanoNat.lt_S_n in Hn1, Hn2. *)
-  apply IH; try lia.
-Admitted. *)
-
-(*NOTE: Working version (mod bound) but with bad hypothesis*)
-(*
-Lemma mk_ts_map_invar gamma pd n1 n2 (s: sort):
-  (forall srts, depth_alt gamma s < n1 srts) ->
-  (forall srts, depth_alt gamma s < n2 srts) ->
-  ts_map_to_pd (fun ts srts => mk_ts_map gamma pd (n1 srts) ts srts) s = 
-  ts_map_to_pd (fun ts srts => mk_ts_map gamma pd (n2 srts) ts srts) s.
-Proof.
-  revert n1 n2.
-  remember (depth_alt gamma s) as n.
-  generalize dependent s.
-  induction n using lt_wf_ind.
-  assert (IH: forall s: sort,
-    depth_alt gamma s < n ->
-    forall n1 n2,
-    (forall srts : list sort, depth_alt gamma s < n1 srts) ->
-    (forall srts : list sort, depth_alt gamma s < n2 srts) ->
-    ts_map_to_pd (fun (ts : typesym) (srts : list sort) => mk_ts_map gamma pd (n1 srts) ts srts) s =
-    ts_map_to_pd (fun (ts : typesym) (srts : list sort) => mk_ts_map gamma pd (n2 srts) ts srts) s).
-  { intros s Hn. apply H; auto. }
-  clear H.
-  intros s Hn n1 n2 Hn1 Hn2. subst.
-  destruct s as [| | ts srts]; simpl; auto.
-  assert (Hn1' := Hn1 srts).
-  assert (Hn2' := Hn2 srts).
-  destruct (n1 srts) as [|n1'] eqn : Hn1s; [lia|].
-  destruct (n2 srts) as [|n2'] eqn : Hn2s; [lia|].
-  simpl.
-  generalize dependent (find_ts_in_ctx_some gamma ts).
-  destruct (find_ts_in_ctx gamma ts) as [[m a]|] eqn : Hfind; auto.
-  intros H. generalize dependent (proj1 (proj2 (H m a eq_refl))).
-  specialize (H m a eq_refl). destruct H as [m_in [a_in Hts]].
-  intros a_in'. assert (a_in' = a_in) by (apply bool_irrelevance). subst. 
-  unfold adt_rep.
-  assert (Hveq: (var_map m srts (ts_map_to_pd (mk_ts_map gamma pd n1'))) = 
-    (var_map m srts (ts_map_to_pd (mk_ts_map gamma pd n2')))). {
-    (*This should be separate lemma*)
-    apply functional_extensionality. intros x.
-    unfold var_map. unfold domain. unfold sigma. unfold ty_subst_s.
-    simpl. 
-    destruct (ty_subst_fun_cases (m_params m) srts s_int x) as [Hin | Hd].
-    + remember (ty_subst_fun (m_params m) srts s_int x) as t.
-      destruct (sort_to_ty t) eqn : Hs; auto.
-      { (*sort not var*) destruct t; simpl in Hs; discriminate. }
-      (*We have to change n1 and n2, but we use the fact that it is bounded (I hope)*)
-      pose proof (depth_alt_in gamma Hin).
-        pose proof (depth_alt_cons_bound gamma (adt_name a) srts).
-      apply (IH t); auto; lia.
-    + rewrite Hd; auto.
-  }
-  rewrite Hveq.
-  (*Now prove typesym_map equality*)
-  erewrite mk_adts_ext; [reflexivity|].
-  intros ts' tys' Hin'. unfold typesym_map.
-  (*So we know (if we change bounds) that sort depth is smaller*)
-  unfold domain. simpl.
-  specialize (IH (s_cons ts' (map (sigma m srts) tys'))).
-  simpl ts_map_to_pd in IH.
-  assert (Hdepth: depth_alt gamma (s_cons ts' (map (sigma m srts) tys')) < depth_alt gamma (s_cons (adt_name a) srts)).
-  {
-    (*Idea: (list_max (map (depth_alt gamma) (map (sigma m srts) tys'))) <=
-      max (list_max (map (depth_alt gamma) srts)) (list_max (map (depth_vty gamma) tys'))
-      by subst properties (maybe we need assumption about params in bounds but that is OK*)
-    (*Then, have that (list_max (map (depth_vty gamma) tys') <= (index typesym_eq_dec ts') by 
-        well-typing of constructors (need valid context) *)
-    (*So, max (index ts') (max (list_map srts) (index ts')) = max (index ts') (max (list_map srts))*)
-    (*And we know that index ts' < index ts', so the result follows*)
-    (*I believe that this should work*)
-    admit.
-  }
-  specialize (IH Hdepth (fun _ => n1') (fun _ => n2')).
-(*   simpl sort_depth in Hn1, Hn2. *)
-  (*Know here that ts' is NON-recursive instance - so it MUST appear BEFORE in gamma*)
-(*  apply PeanoNat.lt_S_n in Hn1, Hn2. *)
-  apply IH; try lia.
-Admitted.*)
-
-(* 
-  - simpl in Hn1, Hn2 |- *.
-    (*Idea: index of ts' is smaller than index of ts, and indices in tys' MUST be 
-      smaller than index of ts as well (by well-typed context)
-      and obviously everythign in srts smaller than srts, so I think we are good
-      *)
-    apply PeanoNat.lt_S_n in Hn1, Hn2.
-    assert ( Hindex: index typesym_eq_dec ts' (typesyms_of_context gamma) < 
-      index typesym_eq_dec ts (typesyms_of_context gamma)). { admit. }
-
-
-      - pose proof (depth_alt_in gamma Hin).
-        pose proof (depth_alt_cons_bound gamma (adt_name a) srts).
-        lia.
-      - intros _. 
-
-
-
-
- simpl.
-      simpl in Hn1, Hn2.
-      pose proof (list_map_map_In_le (depth_alt gamma) Hin).
-      apply IHn1; lia.
-      
-(*       admit. *)
-      (* unfold depth_aux in Hn1, Hn2.
-      simpl in Hn1.
-      simpl sort_depth in Hn1, Hn2.
-      assert (Hn1': list_max (map (sort_depth (constr_depth gamma)) srts) < n1) by nia.
-      assert (Hn2': list_max (map (sort_depth (constr_depth gamma)) srts) < n2) by nia.
-      pose proof (list_map_map_In_le (sort_depth (constr_depth gamma)) Hin). *)
-(*       apply IHn1; lia. *)
-    + rewrite Hd; auto.
-  }
-  
-
- clear H.
-  intros a_in. (*TODO: separate lemma*) unfold adt_rep.
-
-  unfold mk_ts_map.
-  
-  Check PeanoNat.Nat.lt_wf_induction.
-  Check Nat.strong_ind.
-
-  generalize dependent n2. generalize dependent s. induction n1 as [| n1 IHn1].
-  { intros; lia. }
-  intros s [| n2]; [lia | intros Hn1 Hn2].
-  destruct s as [| | ts srts]; simpl; auto.
-  generalize dependent (find_ts_in_ctx_some gamma ts).
-  destruct (find_ts_in_ctx gamma ts) as [[m a]|] eqn : Hfind; auto.
-  intros H. generalize dependent (proj1 (proj2 (H m a eq_refl))). clear H.
-  intros a_in. (*TODO: separate lemma*) unfold adt_rep.
-  assert (Hveq: (var_map m srts (ts_map_to_pd (mk_ts_map gamma pd n1))) = 
-    (var_map m srts (ts_map_to_pd (mk_ts_map gamma pd n2)))). {
-    (*This should be separate lemma*)
-    apply functional_extensionality. intros x.
-    unfold var_map. unfold domain. unfold sigma. simpl. unfold ty_subst_s.
-    simpl. 
-    destruct (ty_subst_fun_cases (m_params m) srts s_int x) as [Hin | Hd].
-    + remember (ty_subst_fun (m_params m) srts s_int x) as t.
-      destruct (sort_to_ty t) eqn : Hs; auto.
-      { (*sort not var*) destruct t; simpl in Hs; discriminate. }
-      simpl in Hn1, Hn2.
-      pose proof (list_map_map_In_le (depth_alt gamma) Hin).
-      apply IHn1; lia.
-      
-(*       admit. *)
-      (* unfold depth_aux in Hn1, Hn2.
-      simpl in Hn1.
-      simpl sort_depth in Hn1, Hn2.
-      assert (Hn1': list_max (map (sort_depth (constr_depth gamma)) srts) < n1) by nia.
-      assert (Hn2': list_max (map (sort_depth (constr_depth gamma)) srts) < n2) by nia.
-      pose proof (list_map_map_In_le (sort_depth (constr_depth gamma)) Hin). *)
-(*       apply IHn1; lia. *)
-    + rewrite Hd; auto.
-  }
-  rewrite Hveq.
-  (*Now prove typesym_map equality*)
-  erewrite mk_adts_ext; [reflexivity|].
-  intros ts' tys' Hin'. unfold typesym_map.
-  (*So we know (if we change bounds) that sort depth is smaller*)
-  unfold domain. simpl.
-  specialize (IHn1 (s_cons ts' (map (sigma m srts) tys')) n2).
-(*   simpl sort_depth in Hn1, Hn2. *)
-  (*Know here that ts' is NON-recursive instance - so it MUST appear BEFORE in gamma*)
-(*  apply PeanoNat.lt_S_n in Hn1, Hn2. *)
-  apply IHn1.
-  - simpl in Hn1, Hn2 |- *.
-    (*Idea: index of ts' is smaller than index of ts, and indices in tys' MUST be 
-      smaller than index of ts as well (by well-typed context)
-      and obviously everythign in srts smaller than srts, so I think we are good
-      *)
-    apply PeanoNat.lt_S_n in Hn1, Hn2.
-    assert ( Hindex: index typesym_eq_dec ts' (typesyms_of_context gamma) < 
-      index typesym_eq_dec ts (typesyms_of_context gamma)). { admit. }
-    (*Idea: (list_max (map (depth_alt gamma) (map (sigma m srts) tys'))) <=
-      max (list_max (map (depth_alt gamma) srts)) (list_max (map (depth_vty gamma) tys'))
-      by subst properties (maybe we need assumption about params in bounds but that is OK*)
-    (*Then, have that (list_max (map (depth_vty gamma) tys') <= (index typesym_eq_dec ts') by 
-        well-typing of constructors (need valid context) *)
-    (*So, max (index ts') (max (list_map srts) (index ts')) = max (index ts') (max (list_map srts))*)
-    (*And we know that index ts' < index ts', so the result follows*)
-    (*I believe that this should work*)
-    admit.
-  - admit.
-Admitted.
-
-Lemma mk_ts_map_invar gamma pd n1 n2 (s: sort):
-  depth_alt gamma s < n1 ->
-  depth_alt gamma s < n2 ->
-  ts_map_to_pd (mk_ts_map gamma pd n1) s = ts_map_to_pd (mk_ts_map gamma pd n2) s.
-Proof.
-  generalize dependent n2. generalize dependent s. induction n1 as [| n1 IHn1].
-  { intros; lia. }
-  intros s [| n2]; [lia | intros Hn1 Hn2].
-  destruct s as [| | ts srts]; simpl; auto.
-  generalize dependent (find_ts_in_ctx_some gamma ts).
-  destruct (find_ts_in_ctx gamma ts) as [[m a]|] eqn : Hfind; auto.
-  intros H. generalize dependent (proj1 (proj2 (H m a eq_refl))). clear H.
-  intros a_in. (*TODO: separate lemma*) unfold adt_rep.
-  assert (Hveq: (var_map m srts (ts_map_to_pd (mk_ts_map gamma pd n1))) = 
-    (var_map m srts (ts_map_to_pd (mk_ts_map gamma pd n2)))). {
-    (*This should be separate lemma*)
-    apply functional_extensionality. intros x.
-    unfold var_map. unfold domain. unfold sigma. simpl. unfold ty_subst_s.
-    simpl. 
-    destruct (ty_subst_fun_cases (m_params m) srts s_int x) as [Hin | Hd].
-    + remember (ty_subst_fun (m_params m) srts s_int x) as t.
-      destruct (sort_to_ty t) eqn : Hs; auto.
-      { (*sort not var*) destruct t; simpl in Hs; discriminate. }
-      simpl in Hn1, Hn2.
-      pose proof (list_map_map_In_le (depth_alt gamma) Hin).
-      apply IHn1; lia.
-      
-(*       admit. *)
-      (* unfold depth_aux in Hn1, Hn2.
-      simpl in Hn1.
-      simpl sort_depth in Hn1, Hn2.
-      assert (Hn1': list_max (map (sort_depth (constr_depth gamma)) srts) < n1) by nia.
-      assert (Hn2': list_max (map (sort_depth (constr_depth gamma)) srts) < n2) by nia.
-      pose proof (list_map_map_In_le (sort_depth (constr_depth gamma)) Hin). *)
-(*       apply IHn1; lia. *)
-    + rewrite Hd; auto.
-  }
-  rewrite Hveq.
-  (*Now prove typesym_map equality*)
-  erewrite mk_adts_ext; [reflexivity|].
-  intros ts' tys' Hin'. unfold typesym_map.
-  (*So we know (if we change bounds) that sort depth is smaller*)
-  unfold domain. simpl.
-  specialize (IHn1 (s_cons ts' (map (sigma m srts) tys')) n2).
-(*   simpl sort_depth in Hn1, Hn2. *)
-  (*Know here that ts' is NON-recursive instance - so it MUST appear BEFORE in gamma*)
-(*  apply PeanoNat.lt_S_n in Hn1, Hn2. *)
-  apply IHn1.
-  - simpl in Hn1, Hn2 |- *.
-    (*Idea: index of ts' is smaller than index of ts, and indices in tys' MUST be 
-      smaller than index of ts as well (by well-typed context)
-      and obviously everythign in srts smaller than srts, so I think we are good
-      *)
-    apply PeanoNat.lt_S_n in Hn1, Hn2.
-    assert ( Hindex: index typesym_eq_dec ts' (typesyms_of_context gamma) < 
-      index typesym_eq_dec ts (typesyms_of_context gamma)). { admit. }
-    (*Idea: (list_max (map (depth_alt gamma) (map (sigma m srts) tys'))) <=
-      max (list_max (map (depth_alt gamma) srts)) (list_max (map (depth_vty gamma) tys'))
-      by subst properties (maybe we need assumption about params in bounds but that is OK*)
-    (*Then, have that (list_max (map (depth_vty gamma) tys') <= (index typesym_eq_dec ts') by 
-        well-typing of constructors (need valid context) *)
-    (*So, max (index ts') (max (list_map srts) (index ts')) = max (index ts') (max (list_map srts))*)
-    (*And we know that index ts' < index ts', so the result follows*)
-    (*I believe that this should work*)
-    admit.
-  - admit.
-Admitted. *)
- (*    lia.
-
- by admit.
-
-    (*Problem is extra +1 - is it actually smaller or could it just be the same?*)
-    (*with + version, can remove the s because ts' is smaller, but then, the max could
-      be as large as max (index ts', srts)*)
-    Search (S ?x < S ?y).
-
-
- (*Idea: index of*) unfold depth_aux in Hn1 |-*. rewrite sort_depth_cons in Hn1 |- *.
-    unfold sigma.
-
-
-
-
-Lemma sorts_depth_bound n srts b
-  (forall x, In x srts -> sort_depth n x < b) ->
-  
-
-Lemma 
-
-
-    rewrite map_map.
-    (*Idea: index ts' < index ts, *)
-
-    
-
- simpl sort_depth.
-
- simpl sort_depth.
-
-    Print sigma.  
-    
-
-  simpl in IHn1.
-
-  Print ts_map_to_pd.
-
-  unfold mk_ts_map.
-  Check mk_ts_map.
-  
-
-
-  destruct (sort_to_ty (typesym_to_sort ts' (seq.map (sigma m srts) tys'))) eqn : Hty; auto.
-  { (*contradiction*) exfalso. apply (var_not_sort t). rewrite <- Hty; auto.
-    destruct (typesym_to_sort ts' (seq.map (sigma m srts) tys')); auto.
-  }
-  (*Idea is that we need to show (ultimately) that this sort is small enough*)
-  apply IHn1.
-  (*TODO: come back once I fix sorts *)
-  admit.
-  admit.
-      * 
-
- unfold sort_to_ty in Hs. 
-        destruct (nth n srts s_int); simpl in Hs; discriminate.
-
-
- destruct (ty_subst_fun (m_params m) srts s_int x) as [| | ts' srts'] eqn : Hty; auto.
-      remember (s_cons ts' srts') as s.
-      unfold ts_map_to_pd in IHn1. apply IHn1.
-      apply IHn1.
-      
-    destruct (in_dec string_dec x (m_params m)) as [Hin| Hin].
-    + (*Case 1: if var in list, maps to corresponding sort, which has smaller size than n1 and n2,
-        so use IH*)
-      (*Note: we need a lemma that doesnt require length eq, as long as in both lists, otherwise prove default
-        for now just admit*)
-      (*TODO: need lemma that says we can find first instance - then case on whether this is in bounds
-        of second or not*)
-     (*  Search In nth.
-      Search index.
-      destruct (In_nth _ _ EmptyString Hin) as [n [Hn Hx]].
-      Search ty_subst_fun List.nth.
-
-
-
-ty_subst_fun_nth_gen:
-  forall {A : Type} (vars : list typevar) (vs : list A) (d : A) (n : nat) (a : typevar) (s : A),
-  n < Datatypes.length vars ->
-  n < Datatypes.length vs -> NoDup vars -> ty_subst_fun vars vs d (nth n vars a) = nth n vs s *)
-
-      destruct (In_nth _ _ EmptyString Hin) as [n [Hn Hx]].
-      subst. unfold ty_subst_s. simpl. rewrite ty_subst_fun_nth with (s:=s_int); auto.
-      2: { (*here*) admit. }
-      2: { apply m_params_Nodup. }
-      destruct (sort_to_ty (nth n srts s_int)) eqn : Hs; auto.
-      { (*sort not var*) unfold sort_to_ty in Hs. 
-        destruct (nth n srts s_int); simpl in Hs; discriminate.
-      }
-      simpl in Hn1, Hn2.
-      apply IHn1.
-      * Search list_max. (*TODO: lemma for In*)
-      unfold ty_subst_s. unfold v_subst. simpl. apply IHn1.
-      * (*identical proofs*)
-        unfold sort_depth. unfold sort_to_srt. simpl.
-        match goal with |- context [ sort_to_srt_aux ?x ?y] => generalize dependent y end.
-        simpl. rewrite !ty_subst_fun_nth with (s:=vty_int); auto.
-        2: { admit. } 2: { apply m_params_Nodup. }
-        unfold sorts_to_tys. rewrite !map_nth_inbound with (d2:=s_int) by admit.
-        (*TODO: this is doable once we have recursive sorts*)
-        admit.
-      * (*similar*) admit.
-    + rewrite !ty_subst_fun_notin; auto.
-  }
-  rewrite Hveq.
-  (*Now prove typesym_map equality*)
-  erewrite mk_adts_ext; [reflexivity|].
-  (*OK, so we need to prove this*)
-  intros ts' tys' Hin'. unfold typesym_map.
-  (*So we know (if we change bounds) that sort depth is smaller*)
-  unfold domain. 
-  destruct (sort_to_ty (typesym_to_sort ts' (seq.map (sigma m srts) tys'))) eqn : Hty; auto.
-  { (*contradiction*) exfalso. apply (var_not_sort t). rewrite <- Hty; auto.
-    destruct (typesym_to_sort ts' (seq.map (sigma m srts) tys')); auto.
-  }
-  (*Idea is that we need to show (ultimately) that this sort is small enough*)
-  apply IHn1.
-  (*TODO: come back once I fix sorts *)
-  admit.
-  admit.
-Admitted.
-
- *)
-
-(*Lemma mk_ts_map_change_n (gamma: context) (pd: sort -> Set) (n1 n2: nat) (ts: typesym) (srts: list sort)
-  (Hn1: sorts_depth srts < n1)
-  (Hn2: sorts_depth srts < n2):
-  mk_ts_map gamma pd n1 ts srts = mk_ts_map gamma pd n2 ts srts.
-Proof.
-  generalize dependent n2. generalize dependent srts. induction n1 as [| n1 IHn1].
-  - intros; lia.
-  - intros srts Hn1 [| n2]; [lia|]; intros Hn2.
-    simpl. generalize dependent (find_ts_in_ctx_some gamma ts).
-    destruct (find_ts_in_ctx gamma ts) as [[m a]|] eqn : Hfind; auto.
-    intros Hdefs. generalize dependent (proj1 (proj2 (Hdefs m a eq_refl))).
-    intros a_in. clear Hdefs.
-    (*Now we need to show we can change adt_rep pd*)
-
-
-
-    (*TODO: separate lemma*)
-    unfold adt_rep.
-    Print mk_adts.
-    Print typesym_map.
-
-Lemma mk_adts_ext (
-    unfold var_map.
-   
-    
-
- specialize (Hdefs m a eq_refl).
-  
-
-Lemma mk_pd_aux_change_n gamma pd n1 n2:*)
-
-(* Check adt_rep.
-Lemma adt_rep_eq m srts pd a a_in:
-  adt_rep' m srts pd pd a a_in = adt_rep m srts pd a a_in.
-Proof. reflexivity. Qed. *)
-
-(*Now we will try to prove for the generalized version*)
-
+(*Now prove that this satisfies [pd_full_aux] for any [n]*)
 Lemma mk_pd_aux_full gamma pd n: valid_context gamma -> pd_full_aux gamma (mk_pd_aux gamma pd n) n.
 Proof.
   intros gamma_valid.
   unfold pd_full_aux, mk_pd_aux. unfold ts_map_to_pd at 1. intros Hn m srts a m_in a_in.
-(*   rewrite sort_rect_typesym_to_sort. *)
-  (*TODO: could I prove that this equals mk_ts ... (pred n) (bc if n large enough, doesn't change)
-    *)
+  (*Idea: we convert [adt_rep] of this function into one with a fixed [n] ([pred (n srts)]).
+    Then we can case on n, unfold, and prove the equality. This uses the invar lemmas above, but
+    we need to repeat parts of the proof*)
   assert (Htest: adt_rep m srts (fun s : sort => ts_map_to_pd (fun ts srts => mk_ts_map gamma pd (n srts) ts srts) s) a a_in =
     adt_rep m srts (fun s : sort => ts_map_to_pd (mk_ts_map gamma pd (pred (n srts))) s) a a_in).
   {
-   (*  pose proof (mk_ts_map_invar' gamma pd (fun x => S (n x)) (S (pred (n srts))) (s_cons (adt_name a) srts)) as Hinvar.
-    prove_hyp Hinvar. { intros x1 x2. specialize (Hn x1 x2); lia. }
-    prove_hyp Hinvar. { specialize (Hn (adt_name a) srts). lia. }
-    simpl in Hinvar. 
-    generalize dependent (find_ts_in_ctx_some gamma (adt_name a)).
-    assert (Hfind: find_ts_in_ctx gamma (adt_name a) = Some (m, a)). {
-      apply find_ts_in_ctx_iff; auto.
-    }
-    rewrite Hfind.
-    intros H.
-    assert (Heq: (proj1 (proj2 (H m a eq_refl))) = a_in) by (apply bool_irrelevance).
-    rewrite Heq. intros Heq1. rewrite <- Heq1.
-
-
- intros Heq1; apply Heq1.
-
- auto.
-
-
-mk_ts_map_invar' *)
-   
-
-    (*maybe we do need another proof here*)
-    (* unfold adt_rep.
-    f_equal.
-    - unfold var_map. apply functional_extensionality. intros x. unfold sigma, ty_subst_s, domain. simpl.
-      Check mk_ts_map_invar.
-
-    apply mk_adts_ext.
-    Search mk_adts. 
-    f_equal.
-
-    Check mk_ts_map_invar.    (*ok, do this later*) *)
-    Check mk_ts_map_invar.
-
     unfold adt_rep.
+    (*Prove var maps eq*)
     assert (Hvar: (var_map m srts
      (fun s : sort =>
       ts_map_to_pd (fun (ts : typesym) (srts0 : list sort) => mk_ts_map gamma pd (n srts0) ts srts0) s)) =
@@ -1858,33 +865,13 @@ mk_ts_map_invar' *)
         * specialize (Hn (adt_name a) srts). lia.
       + rewrite Hd; auto.
     }
-    (*   (var_map m srts
-     (fun s : sort =>
-      ts_map_to_pd
-        (fun (ts : typesym) (srts0 : list sort) => mk_ts_map gamma pd (Init.Nat.pred (n srts0)) ts srts0)
-        s))).
-    { apply functional_extensionality. intros x. unfold var_map. unfold domain, sigma, ty_subst_s. simpl.
-      destruct (ty_subst_fun_cases (m_params m) srts s_int x) as [Hin | Hd].
-      + remember (ty_subst_fun (m_params m) srts s_int x) as t.
-        destruct (sort_to_ty t) as [| | | ts tys] eqn : Hs; auto.
-        { (*sort not var*) destruct t; simpl in Hs; discriminate. }
-        pose proof (depth_alt_in gamma Hin).
-        pose proof (depth_alt_cons_bound gamma (adt_name a) srts).
-        apply mk_ts_map_invar.
-        * intros s. specialize (Hn s). lia.
-        * intros s. specialize (Hn s). lia.
-      + rewrite Hd; auto.
-    } *)
+    (*And typesym maps*)
     rewrite <- Hvar. clear Hvar.
     erewrite mk_adts_ext; [reflexivity|].
     intros ts' tys' Hin'. unfold typesym_map.
-    (*So we know (if we change bounds) that sort depth is smaller*)
     unfold domain. simpl.
     pose proof (mk_ts_map_invar_const gamma_valid pd (n (map (sigma m srts) tys'))
       (Init.Nat.pred (n srts)) (s_cons ts' (map (sigma m srts) tys'))) as Hts.
-
-
-
     assert (Hdepth: size_sort gamma (s_cons ts' (map (sigma m srts) tys')) < size_sort gamma (s_cons (adt_name a) srts)).
     { apply mut_ts_pairs_subst_smaller; auto. } 
     simpl ts_map_to_pd in Hts. apply Hts.
@@ -1892,6 +879,7 @@ mk_ts_map_invar' *)
     - specialize (Hn (adt_name a) srts). lia.
   }
   rewrite Htest. clear Htest.
+  (*We chose [pred(n srts)] before so that when we unfold 1 layer of the LHS (n srts), everything is equal*)
   destruct (n srts) as [| n'] eqn : Hn'.
   - specialize (Hn (adt_name a) srts); lia.
   - simpl. 
@@ -1904,73 +892,9 @@ mk_ts_map_invar' *)
     assert (Heq: (proj1 (proj2 (H m a eq_refl))) = a_in) by (apply bool_irrelevance).
     rewrite Heq. auto.
 Qed.
-(* 
-    simpl in Hts.
-    apply mk_ts_map_invar with (n1:=fun _ => (n (map (sigma m srts) tys')))
-    (n2:= fun _ => (Init.Nat.pred (n (map (sigma m srts) tys')))).
-    Check mk_ts_map_invar.
 
-    specialize (IH (s_cons ts' (map (sigma m srts) tys'))).
-    simpl ts_map_to_pd in IH.
-    assert (Hdepth: depth_alt gamma (s_cons ts' (map (sigma m srts) tys')) < depth_alt gamma (s_cons (adt_name a) srts)).
-    {
-      (*Idea: (list_max (map (depth_alt gamma) (map (sigma m srts) tys'))) <=
-        max (list_max (map (depth_alt gamma) srts)) (list_max (map (depth_vty gamma) tys'))
-        by subst properties (maybe we need assumption about params in bounds but that is OK*)
-      (*Then, have that (list_max (map (depth_vty gamma) tys') <= (index typesym_eq_dec ts') by 
-          well-typing of constructors (need valid context) *)
-      (*So, max (index ts') (max (list_map srts) (index ts')) = max (index ts') (max (list_map srts))*)
-      (*And we know that index ts' < index ts', so the result follows*)
-      (*I believe that this should work*)
-      admit.
-    }
-    specialize (IH Hdepth (fun _ => n1') (fun _ => n2')).
-  (*   simpl sort_depth in Hn1, Hn2. *)
-    (*Know here that ts' is NON-recursive instance - so it MUST appear BEFORE in gamma*)
-  (*  apply PeanoNat.lt_S_n in Hn1, Hn2. *)
-    apply IH; try lia.
-    apply mk_adts_ext.
-
-    pose proof (mk_ts_map_invar gamma pd (fun x => S (n x)) (fun x =>  S (pred (n x))) (s_cons (adt_name a) srts)) as Hts.
-    prove_hyp Hts.
-    { intros s. specialize (Hn s). lia. }
-    prove_hyp Hts. { intros s. specialize (Hn s). lia. }
-    unfold ts_map_to_pd in Hts. simpl in Hts.
-    generalize dependent (find_ts_in_ctx_some gamma (adt_name a)).
-    assert (Hfind: find_ts_in_ctx gamma (adt_name a) = Some (m, a)). {
-      apply find_ts_in_ctx_iff; auto.
-    }
-    rewrite Hfind. intros H. generalize dependent ((proj1 (proj2 (H m a eq_refl)))). clear H.
-    intros a_in'. assert (a_in = a_in') by (apply bool_irrelevance). subst.
-    intros Heq.
-    replace (fun (ts : typesym) (srts0 : list sort) => mk_ts_map gamma pd (n srts0) ts srts0) with
-    (mk_ts_map gamma pd (n srts)).
-    2: { repeat (apply functional_extensionality; intros); auto.
-
- apply Heq. auto.
-  }
-  auto.
-  rewrite Htest. clear Htest.
-  destruct n as [| n'].
-  - intros; lia.
-  - simpl. 
-    generalize dependent (find_ts_in_ctx_some gamma (adt_name a)).
-    assert (Hfind: find_ts_in_ctx gamma (adt_name a) = Some (m, a)). {
-      apply find_ts_in_ctx_iff; auto.
-    }
-    rewrite Hfind.
-    intros H.
-    assert (Heq: (proj1 (proj2 (H m a eq_refl))) = a_in) by (apply bool_irrelevance).
-    rewrite Heq. auto.
-Qed. *)
-
-Check mk_pd_aux_full.
-Print pd_full_aux.
-Print pd_full.
-(* Definition mk_pd' (gamma: context) (pd: sort -> Set) (s: sort) : Set :=
-  mk_pd_aux gamma pd (fun srts => depth_alt gamma s) s. *)
-
-Lemma mk_pd_full gamma pd: valid_context gamma -> pd_full gamma (mk_pd gamma pd).
+(*The full theorem is a simple corollary, since we chose a large enough depth*)
+Theorem mk_pd_full gamma pd: valid_context gamma -> pd_full gamma (mk_pd gamma pd).
 Proof.
   intros gamma_valid. unfold pd_full, mk_pd. intros m srts a m_in a_in.
   apply mk_pd_aux_full; auto.
@@ -1978,7 +902,7 @@ Proof.
 Qed.
 (*The next thing to prove (TODO): for any non-ADT, pd_full gamma (mk_pd gamma pd) = pd*)
 
-
+End InterpProofs.
 (*Going to prove 2 things:
   1. If we assume adts and constrs conditions hold, then we get [adt_interp_props]
   2. We can construct pd and pf st adts and constrs hold by assigning ADT_rep*)
